Added relational Hoare calculus and the link to wp

utp/utp_rel.thy
@@ -239,6 +239,13 @@ definition while :: "'\<alpha> condition \<Rightarrow> '\<alpha> hrelation \<Rig
 
 declare while_def [urel_defs] 
 
+text {* While loops with invariant decoration *}
+
+definition while_inv :: "'\<alpha> condition \<Rightarrow> '\<alpha> condition \<Rightarrow> '\<alpha> hrelation \<Rightarrow> '\<alpha> hrelation" ("while _ invr _ do _ od") where
+"while b invr p do S od = while b do S od"
+
+declare while_inv_def
+
 lemma cond_idem:"(P \<triangleleft> b \<triangleright> P) = P" by rel_tac 
 
 lemma cond_symm:"(P \<triangleleft> b \<triangleright> Q) = (Q \<triangleleft> \<not> b \<triangleright> P)" by rel_tac
@@ -301,6 +308,10 @@ lemma seqr_right_zero [simp]:
 lemma seqr_mono:
   "\<lbrakk> P\<^sub>1 \<sqsubseteq> P\<^sub>2; Q\<^sub>1 \<sqsubseteq> Q\<^sub>2 \<rbrakk> \<Longrightarrow> (P\<^sub>1 ;; Q\<^sub>1) \<sqsubseteq> (P\<^sub>2 ;; Q\<^sub>2)"
   by (rel_tac, blast)
+
+lemma spec_refine:
+  "Q \<sqsubseteq> (P \<and> R) \<Longrightarrow> (P \<Rightarrow> Q) \<sqsubseteq> R"
+  by (rel_tac)
 
 lemma pre_skip_post: "(\<lceil>b\<rceil>\<^sub>< \<and> II) = (II \<and> \<lceil>b\<rceil>\<^sub>>)"
   by (rel_tac)
